simple-frontend/SyntacticTranslation.thy
@@ -2,6 +2,255 @@ theory SyntacticTranslation
   imports FrontEndTranslation
 begin
 
+section \<open>Refinement Calculus\<close>
+
+(* C1 verifies more than C2 *)
+(* If C2 verifies, then C1 verifies as well *)
+(* C1 is more refined *)
+definition verifies_more where
+  "verifies_more \<Delta> C1 C2 \<longleftrightarrow> (\<forall>\<omega> S. stable \<omega> \<and> TypedEqui.typed \<Delta> \<omega> \<and> ConcreteSemantics.red_stmt \<Delta> C2 \<omega> S
+  \<longrightarrow> (\<exists>S'. S' \<subseteq> S \<and> ConcreteSemantics.red_stmt \<Delta> C1 \<omega> S'))"
+
+lemma verifies_moreI:
+  assumes "\<And>\<omega> S'. stable \<omega> \<Longrightarrow> TypedEqui.typed \<Delta> \<omega> \<Longrightarrow> ConcreteSemantics.red_stmt \<Delta> C2 \<omega> S'
+  \<Longrightarrow> (\<exists>S. S \<subseteq> S' \<and> ConcreteSemantics.red_stmt \<Delta> C1 \<omega> S)"
+  shows "verifies_more \<Delta> C1 C2"
+  by (simp add: assms verifies_more_def)
+
+lemma verifies_moreE:
+  assumes "verifies_more \<Delta> C1 C2"
+      and "stable \<omega>"
+      and "TypedEqui.typed \<Delta> \<omega>"
+      and "ConcreteSemantics.red_stmt \<Delta> C2 \<omega> S"
+    shows "\<exists>S'. S' \<subseteq> S \<and> ConcreteSemantics.red_stmt \<Delta> C1 \<omega> S'"
+  by (metis assms(1) assms(2) assms(3) assms(4) verifies_more_def)
+
+lemma verifies_sameI:
+  assumes "\<And>\<omega> S. stable \<omega> \<Longrightarrow> TypedEqui.typed \<Delta> \<omega> \<Longrightarrow> ConcreteSemantics.red_stmt \<Delta> C2 \<omega> S \<Longrightarrow> ConcreteSemantics.red_stmt \<Delta> C1 \<omega> S"
+  shows "verifies_more \<Delta> C1 C2"
+  using assms unfolding verifies_more_def by blast
+
+lemma elim_seq_compo:
+  assumes "ConcreteSemantics.red_stmt \<Delta> (C1 ;; C2) \<omega> S"
+      and "\<And>S1 f. ConcreteSemantics.red_stmt \<Delta> C1 \<omega> S1 \<Longrightarrow> S = \<Union> (f ` S1) \<Longrightarrow> (\<And>\<omega>. \<omega> \<in> S1 \<Longrightarrow> ConcreteSemantics.red_stmt \<Delta> C2 \<omega> (f \<omega>)) \<Longrightarrow> P"
+    shows "P"
+  using assms ConcreteSemantics.red_stmt_Seq_elim ConcreteSemantics.sequential_composition_elim[of \<Delta> _ C2 S]
+  by blast
+
+lemma verifies_more_seq:
+  assumes "verifies_more \<Delta> C1 C1'"
+      and "verifies_more \<Delta> C2 C2'"
+      and "ConcreteSemantics.wf_abs_stmt \<Delta> C1' \<or> ConcreteSemantics.wf_abs_stmt \<Delta> C1"
+    shows "verifies_more \<Delta> (Seq C1 C2) (Seq C1' C2')"
+proof (rule verifies_moreI)
+  fix \<omega> S'
+  assume asm0: "sep_algebra_class.stable \<omega>" "typed \<Delta> \<omega>"
+  assume "ConcreteSemantics.red_stmt \<Delta> (C1' ;; C2') \<omega> S'"
+  then show "\<exists>S. S \<subseteq> S' \<and> ConcreteSemantics.red_stmt \<Delta> (C1 ;; C2) \<omega> S"
+  proof (rule elim_seq_compo)
+    fix S1' f assume asm1: "ConcreteSemantics.red_stmt \<Delta> C1' \<omega> S1'" "S' = \<Union> (f ` S1')"
+      "\<And>\<omega>. \<omega> \<in> S1' \<Longrightarrow> ConcreteSemantics.red_stmt \<Delta> C2' \<omega> (f \<omega>)"
+    then obtain S1 where "ConcreteSemantics.red_stmt \<Delta> C1 \<omega> S1" "S1 \<subseteq> S1'"
+      by (meson asm0(1) asm0(2) assms(1) verifies_moreE)
+
+    let ?f = "\<lambda>\<omega>1. (SOME S2. S2 \<subseteq> f \<omega>1 \<and> ConcreteSemantics.red_stmt \<Delta> C2 \<omega>1 S2)"
+    have r: "\<And>\<omega>1. \<omega>1 \<in> S1 \<Longrightarrow> ?f \<omega>1 \<subseteq> f \<omega>1 \<and> ConcreteSemantics.red_stmt \<Delta> C2 \<omega>1 (?f \<omega>1)"
+    proof -
+      fix \<omega>1 assume "\<omega>1 \<in> S1"
+      then have "TypedEqui.typed \<Delta> \<omega>1 \<and> stable \<omega>1"
+        apply (cases "ConcreteSemantics.wf_abs_stmt \<Delta> C1'")
+        using ConcreteSemantics.red_wf_state TypedEqui.wf_state_def \<open>S1 \<subseteq> S1'\<close> asm0(1) asm0(2) asm1(1) apply blast
+        using ConcreteSemantics.red_wf_state TypedEqui.wf_state_def \<open>ConcreteSemantics.red_stmt \<Delta> C1 \<omega> S1\<close> asm0(1) asm0(2) assms(3) by blast
+      then obtain S2 where "S2 \<subseteq> f \<omega>1" "ConcreteSemantics.red_stmt \<Delta> C2 \<omega>1 S2"
+        by (meson \<open>S1 \<subseteq> S1'\<close> \<open>\<omega>1 \<in> S1\<close> asm1(3) assms(2) in_mono verifies_moreE)
+      then show "?f \<omega>1 \<subseteq> f \<omega>1 \<and> ConcreteSemantics.red_stmt \<Delta> C2 \<omega>1 (?f \<omega>1)"
+        by (metis (mono_tags, lifting) someI2_ex)
+    qed
+
+    let ?S = "\<Union> (?f ` S1)"
+    have "?S \<subseteq> S'"
+      by (simp add: SUP_subset_mono \<open>S1 \<subseteq> S1'\<close> asm1(2) r)
+    moreover have "ConcreteSemantics.red_stmt \<Delta> (C1 ;; C2) \<omega> ?S"
+      using \<open>ConcreteSemantics.red_stmt \<Delta> C1 \<omega> S1\<close>
+    proof (rule ConcreteSemantics.RedSeq)
+      show "ConcreteSemantics.sequential_composition \<Delta> S1 C2 (\<Union>\<omega>1\<in>S1. SOME S2. S2 \<subseteq> f \<omega>1 \<and> ConcreteSemantics.red_stmt \<Delta> C2 \<omega>1 S2)"
+        by (metis (no_types, lifting) ConcreteSemantics.red_stmt_sequential_composition.intros(1) r)
+    qed
+    ultimately show "\<exists>S\<subseteq>S'. ConcreteSemantics.red_stmt \<Delta> (C1 ;; C2) \<omega> S"
+      by meson
+  qed
+qed
+
+(* everything accepted by e' is also accepted by e *)
+definition exp_refined_by where
+  "exp_refined_by \<Delta> e e' = (\<forall>\<omega> v. sep_algebra_class.stable \<omega> \<and> typed \<Delta> \<omega> \<and> e' \<omega> = Some v \<longrightarrow> e \<omega> = Some v)"
+
+lemma exp_refined_byI:
+  assumes "\<And>\<omega> v. sep_algebra_class.stable \<omega> \<Longrightarrow> typed \<Delta> \<omega> \<Longrightarrow> e' \<omega> = Some v \<Longrightarrow> e \<omega> = Some v"
+  shows "exp_refined_by \<Delta> e e'"
+  by (simp add: assms exp_refined_by_def)
+
+lemma exp_refined_byE:
+  assumes "exp_refined_by \<Delta> e e'"
+      and "sep_algebra_class.stable \<omega>"
+      and "typed \<Delta> \<omega>"
+      and "e' \<omega> = Some v"
+    shows "e \<omega> = Some v"
+  by (meson assms(1) assms(2) assms(3) assms(4) exp_refined_by_def)
+
+lemma exp_refined_by_refl[simp]:
+  "exp_refined_by \<Delta> e e"
+  using exp_refined_by_def by blast
+
+
+lemma verifies_more_if:
+  assumes "verifies_more \<Delta> C1 C1'"
+      and "verifies_more \<Delta> C2 C2'"
+      and "exp_refined_by \<Delta> b b'"
+    shows "verifies_more \<Delta> (If b C1 C2) (If b' C1' C2')"
+proof (rule verifies_moreI)
+  fix \<omega> S'
+  assume asm0: "sep_algebra_class.stable \<omega>" "typed \<Delta> \<omega>"
+  assume "ConcreteSemantics.red_stmt \<Delta> (abs_stmt.If b' C1' C2') \<omega> S'"
+  then show "\<exists>S\<subseteq>S'. ConcreteSemantics.red_stmt \<Delta> (abs_stmt.If b C1 C2) \<omega> S"
+  proof (rule ConcreteSemantics.red_stmt_If_elim)
+    assume "b' \<omega> = Some True" "ConcreteSemantics.red_stmt \<Delta> C1' \<omega> S'"
+    then obtain S where "S \<subseteq> S'" "ConcreteSemantics.red_stmt \<Delta> C1 \<omega> S"
+      by (meson asm0(1) asm0(2) assms(1) verifies_moreE)
+    moreover have "b \<omega> = Some True"
+      using assms(3) unfolding exp_refined_by_def
+      using \<open>b' \<omega> = Some True\<close> asm0(1) asm0(2) by blast
+    ultimately show "\<exists>S\<subseteq>S'. ConcreteSemantics.red_stmt \<Delta> (abs_stmt.If b C1 C2) \<omega> S"
+      by (meson ConcreteSemantics.RedIfTrue)
+  next
+    assume "b' \<omega> = Some False" "ConcreteSemantics.red_stmt \<Delta> C2' \<omega> S'"
+    then obtain S where "S \<subseteq> S'" "ConcreteSemantics.red_stmt \<Delta> C2 \<omega> S"
+      by (meson asm0(1) asm0(2) assms(2) verifies_moreE)
+    moreover have "b \<omega> = Some False"
+      by (meson \<open>b' \<omega> = Some False\<close> asm0(1) asm0(2) assms(3) exp_refined_by_def)
+    ultimately show "\<exists>S\<subseteq>S'. ConcreteSemantics.red_stmt \<Delta> (abs_stmt.If b C1 C2) \<omega> S"
+      by (meson ConcreteSemantics.RedIfFalse)
+  qed
+qed
+
+
+(* for havoc and skip *)
+lemma verifies_more_refl[simp]:
+  "verifies_more \<Delta> C C"
+  using verifies_sameI by blast
+
+lemma verifies_more_trans:
+  assumes "verifies_more \<Delta> C1 C2"
+      and "verifies_more \<Delta> C2 C3"
+    shows "verifies_more \<Delta> C1 C3"
+proof (rule verifies_moreI)
+  fix \<omega> S3
+  assume "sep_algebra_class.stable \<omega>" "typed \<Delta> \<omega>" "ConcreteSemantics.red_stmt \<Delta> C3 \<omega> S3"
+  then obtain S2 where "S2 \<subseteq> S3" "ConcreteSemantics.red_stmt \<Delta> C2 \<omega> S2"
+    by (meson assms(2) verifies_moreE)
+  then show "\<exists>S\<subseteq>S3. ConcreteSemantics.red_stmt \<Delta> C1 \<omega> S"
+    by (meson \<open>sep_algebra_class.stable \<omega>\<close> \<open>typed \<Delta> \<omega>\<close> assms(1) dual_order.trans verifies_moreE)
+qed
+
+lemma verifies_more_local_assign:
+  assumes "exp_refined_by \<Delta> e e'"
+  shows "verifies_more \<Delta> (LocalAssign x e) (LocalAssign x e')"
+  apply (rule verifies_moreI)
+  using assms unfolding exp_refined_by_def
+  by (metis ConcreteSemantics.RedLocalAssign ConcreteSemantics.red_stmt_Assign_elim equalityE)
+
+lemma verifies_more_exhale:
+  assumes "\<And>a. typed \<Delta> a \<Longrightarrow> a \<in> A' \<Longrightarrow> a \<in> A"
+(* Weaker than A' \<subseteq> A *)
+(* assumes "\<And>\<omega>' \<omega> a. sep_algebra_class.stable \<omega> \<Longrightarrow> typed \<Delta> \<omega> \<Longrightarrow> a \<in> A' \<Longrightarrow> Some \<omega> = \<omega>' \<oplus> a \<Longrightarrow> sep_algebra_class.stable \<omega>' \<Longrightarrow> a \<in> A" *)
+  shows "verifies_more \<Delta> (Exhale A) (Exhale A')"
+proof (rule verifies_moreI)
+  fix \<omega> S'
+  assume asm0: "sep_algebra_class.stable \<omega>" "typed \<Delta> \<omega>"
+  assume "ConcreteSemantics.red_stmt \<Delta> (abs_stmt.Exhale A') \<omega> S'"
+  then show "\<exists>S\<subseteq>S'. ConcreteSemantics.red_stmt \<Delta> (abs_stmt.Exhale A) \<omega> S"
+  proof (rule ConcreteSemantics.red_stmt_Exhale_elim)
+    fix a \<omega>'
+    assume asm1: "S' = {\<omega>'}" "a \<in> A'" "Some \<omega> = \<omega>' \<oplus> a" "sep_algebra_class.stable \<omega>'"
+    then have "a \<in> A" using assms(1)
+      using TypedEqui.typed_smaller asm0(2) greater_equiv by blast
+    then show "\<exists>S\<subseteq>S'. ConcreteSemantics.red_stmt \<Delta> (abs_stmt.Exhale A) \<omega> S"
+      by (metis ConcreteSemantics.semantics_axioms asm1(1) asm1(3) asm1(4) dual_order.refl semantics.RedExhale)
+  qed
+qed
+
+
+lemma verifies_more_inhale_complex:
+  assumes "\<And>\<omega>. sep_algebra_class.stable \<omega> \<Longrightarrow> typed \<Delta> \<omega> \<Longrightarrow> rel_stable_assertion \<omega> A' \<Longrightarrow> rel_stable_assertion \<omega> A"
+      and "\<And>\<omega>' \<omega> a. sep_algebra_class.stable \<omega> \<Longrightarrow> a \<in> A \<Longrightarrow> Some \<omega>' = \<omega> \<oplus> a \<Longrightarrow> 
+sep_algebra_class.stable \<omega>' \<Longrightarrow> typed \<Delta> \<omega>' \<Longrightarrow> (\<exists>a' \<in> A'. Some \<omega>' = \<omega> \<oplus> a')"
+  shows "verifies_more \<Delta> (Inhale A) (Inhale A')"
+proof (rule verifies_moreI)
+  fix \<omega> S'
+  assume asm0: "sep_algebra_class.stable \<omega>" "typed \<Delta> \<omega>"
+  assume "ConcreteSemantics.red_stmt \<Delta> (abs_stmt.Inhale A') \<omega> S'"
+  then show "\<exists>S\<subseteq>S'. ConcreteSemantics.red_stmt \<Delta> (abs_stmt.Inhale A) \<omega> S"
+  proof (rule ConcreteSemantics.red_stmt_Inhale_elim)
+    assume asm1: "S' = Set.filter (\<lambda>\<omega>. sep_algebra_class.stable \<omega> \<and> typed \<Delta> \<omega>) ({\<omega>} \<otimes> A')"
+      "rel_stable_assertion \<omega> A'"
+    then have "ConcreteSemantics.red_stmt \<Delta> (abs_stmt.Inhale A) \<omega> (Set.filter (\<lambda>\<omega>. sep_algebra_class.stable \<omega> \<and> typed \<Delta> \<omega>) ({\<omega>} \<otimes> A))"
+      by (simp add: ConcreteSemantics.RedInhale asm0(1) asm0(2) assms(1))
+    moreover have "Set.filter (\<lambda>\<omega>. sep_algebra_class.stable \<omega> \<and> typed \<Delta> \<omega>) ({\<omega>} \<otimes> A) \<subseteq> Set.filter (\<lambda>\<omega>. sep_algebra_class.stable \<omega> \<and> typed \<Delta> \<omega>) ({\<omega>} \<otimes> A')"
+      by (smt (verit, ccfv_SIG) asm0(1) assms(2) member_filter singletonD subsetI x_elem_set_product)
+    ultimately show "\<exists>S\<subseteq>S'. ConcreteSemantics.red_stmt \<Delta> (abs_stmt.Inhale A) \<omega> S"
+      by (metis (no_types, lifting) asm1(1))
+  qed
+qed
+
+lemma verifies_more_inhale:
+  assumes "\<And>\<omega>. sep_algebra_class.stable \<omega> \<Longrightarrow> typed \<Delta> \<omega> \<Longrightarrow> rel_stable_assertion \<omega> A' \<Longrightarrow> rel_stable_assertion \<omega> A"
+      and "\<And>a. typed \<Delta> a \<Longrightarrow> a \<in> A \<Longrightarrow> a \<in> A'"
+(* Weaker than A \<subseteq> A' *)
+    shows "verifies_more \<Delta> (Inhale A) (Inhale A')"
+proof (rule verifies_more_inhale_complex)
+  show "\<And>\<omega>' \<omega> a. sep_algebra_class.stable \<omega> \<Longrightarrow> a \<in> A \<Longrightarrow> Some \<omega>' = \<omega> \<oplus> a \<Longrightarrow> sep_algebra_class.stable \<omega>' \<Longrightarrow> typed \<Delta> \<omega>' \<Longrightarrow> \<exists>a'\<in>A'. Some \<omega>' = \<omega> \<oplus> a'"
+    using TypedEqui.typed_smaller assms(2) greater_equiv by blast
+qed (simp add: assms(1))
+
+lemma verifies_more_field_assign:
+  assumes "exp_refined_by \<Delta> r r'"
+      and "exp_refined_by \<Delta> e e'"
+  shows "verifies_more \<Delta> (Custom (FieldAssign r f e)) (Custom (FieldAssign r' f e'))"
+proof (rule verifies_moreI)
+  fix \<omega> S'
+  assume asm0: "sep_algebra_class.stable \<omega>" "typed \<Delta> \<omega>"
+  assume "ConcreteSemantics.red_stmt \<Delta> (Custom (custom.FieldAssign r' f e')) \<omega> S'"
+  then show "\<exists>S\<subseteq>S'. ConcreteSemantics.red_stmt \<Delta> (Custom (custom.FieldAssign r f e)) \<omega> S"
+  proof (rule ConcreteSemantics.red_stmt_Custom_elim)
+    assume "red_custom_stmt \<Delta> (custom.FieldAssign r' f e') \<omega> S'"
+    then show "\<exists>S\<subseteq>S'. ConcreteSemantics.red_stmt \<Delta> (Custom (custom.FieldAssign r f e)) \<omega> S"
+    proof (rule red_custom_stmt_FieldAssign)
+      fix hl v ty
+      assume asm1: "S' = {update_heap_val \<omega> (hl, f) v}" "r' \<omega> = Some hl" "e' \<omega> = Some v" "get_m \<omega> (hl, f) = 1"
+        "custom_context \<Delta> f = Some ty" "v \<in> ty"
+      then have "r \<omega> = Some hl \<and> e \<omega> = Some v"
+        using asm0(1) asm0(2) assms(1) assms(2) exp_refined_by_def by metis
+      then show "\<exists>S\<subseteq>S'. ConcreteSemantics.red_stmt \<Delta> (Custom (custom.FieldAssign r f e)) \<omega> S"
+        by (metis ConcreteSemantics.RedCustom Orderings.order_eq_iff RedFieldAssign asm1(1) asm1(4) asm1(5) asm1(6))
+    qed
+  qed
+qed
+
+
+
+
+
+
+
+
+
+section \<open>Syntactic Translation\<close>
+
+(* Goal: Show that if syntactic translation verifies, then the "semantic" translation also verifies *)
+(* verifies_more semantic syntactic *)
+(* exp_refined_by semantic syntactic *)
+
+
 fun translate_binop :: "int_binop \<Rightarrow> binop" where
   "translate_binop Add = binop.Add"
 | "translate_binop Sub = binop.Sub"
@@ -15,76 +264,128 @@ fun translate_exp where
 fun translate_bexp where
   "translate_bexp (Beq e1 e2) = Binop (translate_exp e1) Eq (translate_exp e2)"
 | "translate_bexp (Band e1 e2) = Binop (translate_bexp e1) And (translate_bexp e2)"
-| "translate_bexp (Bnot e) = Unop Not (translate_bexp e)"
+| "translate_bexp (Bnot b) = Unop Not (translate_bexp b)"
 
-(*
-record ('v, 'a) interp =
-  domains :: "'v \<Rightarrow> abs_type"
-  predicates :: "'v predicate_loc \<rightharpoonup> 'a set"
-  funs :: "function_ident \<Rightarrow> 'v val list \<Rightarrow> 'a \<rightharpoonup> 'v val"
+fun typed_exp where
+  "typed_exp (Elit l) \<longleftrightarrow> True"
+| "typed_exp (Evar x) \<longleftrightarrow> (x < undefined \<and> x mod 2 = 0)"
+| "typed_exp (Ebinop e1 op e2) \<longleftrightarrow> typed_exp e1 \<and> typed_exp e2"
 
-record ('v, 'c) abs_type_context =
-  variables :: "var \<rightharpoonup> 'v abs_vtyp"
-  custom_context :: 'c
-*)
-(*
-custom_context \<Delta> = type_ctxt_heap
-*)
-(*
-lemma translation_correct_exp:
-  assumes "TypedEqui.typed type_ctxt_front_end \<omega>"
-(* Also needs something about typed program! *)
-  shows "make_semantic_exp \<Delta> (translate_exp e) \<omega> = semantify_exp e \<omega>"
-  unfolding make_semantic_exp_def semantify_exp_def
-proof (induct e)
-  case (Evar x)
-(* One can be none, the other one not... *)
-  then show ?case sorry
-next
-  case (Elit x)
-  show ?case sorry
-(*
-  proof (rule ext)
-    fix \<omega>
-    have "(if \<exists>v. \<Delta> \<turnstile> \<langle>translate_exp (Elit x);\<omega>\<rangle> [\<Down>] Val v then Some (SOME v. \<Delta> \<turnstile> \<langle>translate_exp (Elit x);\<omega>\<rangle> [\<Down>] Val v) else None)
-      = Some (SOME v. \<Delta> \<turnstile> \<langle>translate_exp (Elit x);\<omega>\<rangle> [\<Down>] Val v)"
-      by (metis RedLit translate_exp.simps(2))
-    also have "... = Some (VInt x)"
-      using someI[of "\<lambda>v. \<Delta> \<turnstile> \<langle>translate_exp (Elit x);\<omega>\<rangle> [\<Down>] Val v" "VInt x"]
-    proof -
-      have "\<Delta> \<turnstile> \<langle>translate_exp (Elit x);\<omega>\<rangle> [\<Down>] Val (VInt x)"
-        by (metis RedLitInt2Val_case calculation option.distinct(1) translate_exp.simps(2) val_of_lit.simps(2))
-      then have "\<Delta> \<turnstile> \<langle>translate_exp (Elit x);\<omega>\<rangle> [\<Down>] Val (SOME v. \<Delta> \<turnstile> \<langle>translate_exp (Elit x);\<omega>\<rangle> [\<Down>] Val v)"
-        using someI by metis
-      then show ?thesis
-        using \<open>\<Delta> \<turnstile> \<langle>translate_exp (Elit x);\<omega>\<rangle> [\<Down>] Val (VInt x)\<close> red_pure_val_unique(1) by blast
-    qed
-    finally show "(if \<exists>v. \<Delta> \<turnstile> \<langle>translate_exp (Elit x);\<omega>\<rangle> [\<Down>] Val v then Some (SOME v. \<Delta> \<turnstile> \<langle>translate_exp (Elit x);\<omega>\<rangle> [\<Down>] Val v) else None) =
-         Some (VInt (edenot (Elit x) (get_store \<omega>)))"
-      by fastforce
+fun typed_bexp where
+  "typed_bexp (Beq e1 e2) \<longleftrightarrow> typed_exp e1 \<and> typed_exp e2"
+| "typed_bexp (Band b1 b2) \<longleftrightarrow> typed_bexp b1 \<and> typed_bexp b2"
+| "typed_bexp (Bnot b) \<longleftrightarrow> typed_bexp b"
+
+fun typed_stmt where
+  "typed_stmt Cskip \<longleftrightarrow> True"
+| "typed_stmt (Cassign x e) \<longleftrightarrow> typed_exp e"
+| "typed_stmt (Cseq C1 C2) \<longleftrightarrow> typed_stmt C1 \<and> typed_stmt C2"
+| "typed_stmt (Cif b C1 C2) \<longleftrightarrow> typed_bexp b \<and> typed_stmt C1 \<and> typed_stmt C2"
+| "typed_stmt (Calloc r e) \<longleftrightarrow> typed_exp e"
+| "typed_stmt (Cwrite r e) \<longleftrightarrow> typed_exp e"
+| "typed_stmt (Cfree r) \<longleftrightarrow> True"
+| "typed_stmt (Cread x r) \<longleftrightarrow> True"
+| "typed_stmt (Cwhile b _ C) \<longleftrightarrow> typed_bexp b \<and> typed_stmt C"
+| "typed_stmt ({_} C1 {_} || {_} C2 {_}) \<longleftrightarrow> typed_stmt C1 \<and> typed_stmt C2"
+
+lemma exp_refined_by_int:
+  assumes "typed_exp e"
+  shows "exp_refined_by tcfe (semantify_exp e) (make_semantic_exp \<Delta> (translate_exp e))"
+proof (rule exp_refined_byI)
+  fix \<omega> v assume "sep_algebra_class.stable \<omega>" "typed tcfe \<omega>"
+  then have asm0: "store_typed (variables tcfe) (get_store \<omega>)"
+    using TypedEqui.typed_def TypedEqui.typed_store_def by blast
+
+  have "typed_exp e \<Longrightarrow> make_semantic_exp \<Delta> (translate_exp e) \<omega> = Some v \<Longrightarrow> semantify_exp e \<omega> = Some v"
+  proof (induct e arbitrary: v)
+    case (Evar x)
+    then have "variables tcfe x = Some vints"
+      by (simp add: type_ctxt_front_end_def type_ctxt_store_def)
+    then obtain v' where "get_store \<omega> x = Some v'" "v' \<in> vints"
+      using asm0 store_typed_lookup by blast
+    then show ?case
+      by (smt (verit) CollectD Evar.prems(2) RedVar2Val_case edenot.simps(1) make_semantic_exp_Some option.sel semantify_exp_def translate_exp.simps(1) val.sel(1) vints_def)
+  next
+    case (Elit x)
+    then show ?case
+      by (metis RedLitInt2Val_case edenot.simps(2) make_semantic_exp_Some semantify_exp_def translate_exp.simps(2) val_of_lit.simps(2))
+  next
+    case (Ebinop e1 op e2)
+    then show ?case
+      by (cases "op"; clarsimp simp add:semantify_exp_def red_pure_simps; fastforce)
   qed
-*)
-next
-  case (Ebinop e1 bop e2)
-  then show ?case sorry
+  then show "make_semantic_exp \<Delta> (translate_exp e) \<omega> = Some v \<Longrightarrow> semantify_exp e \<omega> = Some v" using assms by blast
 qed
 
-lemma translation_correct_bexp:
-  assumes "TypedEqui.typed type_ctxt_front_end \<omega>"
-(* Also needs something about typed program! *)
-  shows "make_semantic_bexp \<Delta> (translate_bexp e) \<omega> = semantify_bexp e \<omega>"
-  unfolding make_semantic_bexp_def semantify_bexp_def
-proof (induct e)
-  case (Beq e1 e2)
-  then show ?case sorry
-next
-  case (Band e1 e2)
-  then show ?case sorry
-next
-  case (Bnot e)
-  then show ?case sorry
+lemma semantify_bexp_band:
+  assumes "make_semantic_bexp \<Delta> (Binop b1 And b2)  \<omega> = Some v"
+  shows "\<exists>v1 v2. v = (v1 \<and> v2) \<and> make_semantic_bexp \<Delta> b1 \<omega> = Some v1 \<and> make_semantic_bexp \<Delta> b2 \<omega> = Some v2"
+  sorry (* TODO: Do on the same model as semantify_bexp_bnot *)
+
+
+lemma semantify_bexp_bnot:
+  assumes "make_semantic_bexp \<Delta> (Unop Not b)  \<omega> = Some v"
+  shows "make_semantic_bexp \<Delta> b \<omega> = Some (\<not> v)"
+proof (cases "\<Delta> \<turnstile> \<langle>Unop Not b; \<omega>\<rangle> [\<Down>] Val (VBool True)")
+  case True
+  then show ?thesis
+    apply (rule red_pure_elim(3))
+    apply (smt (z3) True assms binop_result.inject binop_result.simps(4) eval_unop.elims make_semantic_bexp_Some unop.simps(1))
+    by auto
+  next
+    case False
+    then have "\<Delta> \<turnstile> \<langle>Unop Not b; \<omega>\<rangle> [\<Down>] Val (VBool False)"
+      by (metis (full_types) assms make_semantic_bexp_Some)
+    then show ?thesis
+    proof (rule red_pure_elim(3))
+      fix va v'
+      assume "Val (VBool False) = Val v'" "\<Delta> \<turnstile> \<langle>b;\<omega>\<rangle> [\<Down>] Val va" "eval_unop unop.Not va = BinopNormal v'"
+      then have "v' = VBool False \<and> va = VBool True"
+        using eval_unop.elims by auto
+      then show "make_semantic_bexp \<Delta> b \<omega> = Some (\<not> v)"
+        by (metis (full_types) False \<open>\<Delta> \<turnstile> \<langle>b;\<omega>\<rangle> [\<Down>] Val va\<close> assms make_semantic_bexp_Some)
+    qed (simp)
 qed
-*)
+
+
+lemma semantify_bexp_beq:
+  assumes "make_semantic_bexp \<Delta> (Binop e1 Eq e2)  \<omega> = Some v"
+  shows "\<exists>v1 v2. v = (v1 = v2) \<and> make_semantic_exp \<Delta> e1 \<omega> = Some v1 \<and> make_semantic_exp \<Delta> e2 \<omega> = Some v2"
+  sorry (* TODO: Do on the same model as semantify_bexp_bnot *)
+
+lemma bexp_refined_by:
+  assumes "typed_bexp b"
+  shows "exp_refined_by tcfe (semantify_bexp b) (make_semantic_bexp \<Delta> (translate_bexp b))"
+proof (rule exp_refined_byI)
+  fix \<omega> v assume asm0: "sep_algebra_class.stable \<omega>" "typed tcfe \<omega>"
+  have "typed_bexp b \<Longrightarrow> make_semantic_bexp \<Delta> (translate_bexp b) \<omega> = Some v \<Longrightarrow> semantify_bexp b \<omega> = Some v"
+  proof (induct b arbitrary: v)
+    case (Beq e1 e2)
+    then obtain v1 v2 where "v = (v1 = v2)" "make_semantic_exp \<Delta> (translate_exp e1) \<omega> = Some v1"
+      "make_semantic_exp \<Delta> (translate_exp e2) \<omega> = Some v2"
+      by (smt (z3) semantify_bexp_beq translate_bexp.simps(1))
+    then have "semantify_exp e1 \<omega> = Some v1 \<and> semantify_exp e2 \<omega> = Some v2"
+      by (meson Beq.prems(1) asm0(1) asm0(2) exp_refined_byE exp_refined_by_int typed_bexp.simps(1))
+    then show ?case
+      using \<open>\<And>thesis. (\<And>v1 v2. \<lbrakk>v = (v1 = v2); make_semantic_exp \<Delta> (translate_exp e1) \<omega> = Some v1; make_semantic_exp \<Delta> (translate_exp e2) \<omega> = Some v2\<rbrakk> \<Longrightarrow> thesis) \<Longrightarrow> thesis\<close> \<open>make_semantic_exp \<Delta> (translate_exp e1) \<omega> = Some v1\<close> \<open>make_semantic_exp \<Delta> (translate_exp e2) \<omega> = Some v2\<close> semantify_bexp_def semantify_exp_def by auto
+  next
+    case (Band b1 b2)
+    then obtain v1 v2 where "v = (v1 \<and> v2)" "make_semantic_bexp \<Delta> (translate_bexp b1) \<omega> = Some v1"
+      "make_semantic_bexp \<Delta> (translate_bexp b2) \<omega> = Some v2"
+      by (smt (z3) semantify_bexp_band translate_bexp.simps(2))
+    then show ?case 
+      by (smt (verit) Band.hyps(1) Band.hyps(2) Band.prems(1) bdenot.simps(2) semantify_bexp_def typed_bexp.simps(2))
+  next
+    case (Bnot b)
+    then have "make_semantic_bexp \<Delta> (translate_bexp b) \<omega> = Some (\<not> v)"
+      by (metis semantify_bexp_bnot translate_bexp.simps(3))
+    then show ?case
+      by (metis (full_types) Bnot.hyps Bnot.prems(1) bdenot.simps(3) semantify_bexp_def typed_bexp.simps(3))
+  qed
+  then show "make_semantic_bexp \<Delta> (translate_bexp b) \<omega> = Some v \<Longrightarrow> semantify_bexp b \<omega> = Some v" using assms by blast
+qed
+
+
 definition syntactic_translate_addr :: "var \<Rightarrow> pure_exp" where
   "syntactic_translate_addr r = Var r"
 
@@ -108,116 +409,16 @@ proof (rule ext)
 qed
 
 lemma make_semantic_star:
-  "make_semantic_assertion \<Delta> F (A && B) = make_semantic_assertion \<Delta> F A \<otimes> make_semantic_assertion \<Delta> F B"
-  by (simp add: make_semantic_assertion_def well_typedly_add_set)
+  "make_semantic_assertion_untyped \<Delta> F (A && B) = make_semantic_assertion_untyped \<Delta> F A \<otimes> make_semantic_assertion_untyped \<Delta> F B"
+  by (simp add: make_semantic_assertion_gen_def)
 
-lemma make_semantic_inter_1:
-  "make_semantic_assertion \<Delta> F (I && Atomic (Pure (Unop Not (translate_bexp b)))) = (make_semantic_assertion \<Delta> F I) \<inter> assertify_bexp (Bnot b)"
-  sorry
 
-(*
-lemma make_semantic_inter_2:
-  "make_semantic_assertion \<Delta> type_ctxt_front_end_syntactic (I && Atomic (Pure (translate_bexp b))) = (make_semantic_assertion \<Delta> type_ctxt_front_end_syntactic I) \<inter> assertify_bexp b"
-proof
-  show "make_semantic_assertion \<Delta> type_ctxt_front_end_syntactic (I && Atomic (Pure (translate_bexp b))) \<subseteq> make_semantic_assertion \<Delta> type_ctxt_front_end_syntactic I \<inter> assertify_bexp b"
-    unfolding make_semantic_assertion_def well_typedly_def
-  proof
-    fix \<omega> assume "\<omega> \<in> Set.filter (typed (make_context_semantic \<Delta> type_ctxt_front_end_syntactic)) (\<langle>\<Delta>, snd type_ctxt_front_end_syntactic\<rangle> \<Turnstile> \<langle>I && Atomic (Pure (translate_bexp b))\<rangle>)"
-    then obtain i p where ip: "Some \<omega> = i \<oplus> p" "i \<in> \<langle>\<Delta>, snd type_ctxt_front_end_syntactic\<rangle> \<Turnstile> \<langle>I\<rangle>" "p \<in> \<langle>\<Delta>, snd type_ctxt_front_end_syntactic\<rangle> \<Turnstile> \<langle>Atomic (Pure (translate_bexp b))\<rangle>"     
-      by (smt (verit, ccfv_threshold) member_filter sat_set.simps(4) snd_conv type_ctxt_front_end_syntactic_def x_elem_set_product)
-    then have "pure p"
-      by (metis CollectD Instantiation.atomic_assert.simps(1) Int_iff corely_def emp_core_def red_pure_assert_def sat_set.simps(1))
-    then have "\<omega> \<in> \<langle>\<Delta>, snd type_ctxt_front_end_syntactic\<rangle> \<Turnstile> \<langle>I\<rangle>"
-      using ip(1-2)
-      sorry (* TODO: Prove *)
-    moreover have "get_store \<omega> = get_store p"
-      by (metis \<open>Some \<omega> = i \<oplus> p\<close> commutative full_add_charact(1))
-    moreover have "typed type_ctxt_front_end \<omega>" using make_context_semantic_type_ctxt
-      by (metis \<open>\<omega> \<in> Set.filter (typed (make_context_semantic \<Delta> type_ctxt_front_end_syntactic)) (\<langle>\<Delta>, snd type_ctxt_front_end_syntactic\<rangle> \<Turnstile> \<langle>I && Atomic (Pure (translate_bexp b))\<rangle>)\<close> member_filter)
-    then have "TypedEqui.typed type_ctxt_front_end p"
-      by (metis TypedEqui.typed_smaller commutative greater_def ip(1))
-    then have "bdenot b (get_store p)"
-      using translation_correct_bexp[of p _ b] ip(3)
-      unfolding semantify_bexp_def make_semantic_bexp_def assertify_bexp_def sat_set.simps atomic_assert.simps red_pure_assert_def
-        corely_def
-      by (metis Int_Collect inf.commute option.inject)
-    ultimately have "\<omega> \<in> assertify_bexp b"
-      using translation_correct_bexp[of _ _ b] ip(3) unfolding semantify_bexp_def make_semantic_bexp_def assertify_bexp_def
-      by simp
-    then show "\<omega> \<in> Set.filter (typed (make_context_semantic \<Delta> type_ctxt_front_end_syntactic)) (\<langle>\<Delta>, snd type_ctxt_front_end_syntactic\<rangle> \<Turnstile> \<langle>I\<rangle>) \<inter> assertify_bexp b"
-      by (simp add: \<open>\<omega> \<in> \<langle>\<Delta>, snd type_ctxt_front_end_syntactic\<rangle> \<Turnstile> \<langle>I\<rangle>\<close> \<open>typed type_ctxt_front_end \<omega>\<close> make_context_semantic_type_ctxt)
-  qed
-  show "make_semantic_assertion \<Delta> type_ctxt_front_end_syntactic I \<inter> assertify_bexp b
-    \<subseteq> make_semantic_assertion \<Delta> type_ctxt_front_end_syntactic (I && Atomic (Pure (translate_bexp b)))"
-    unfolding make_semantic_assertion_def assertify_bexp_def well_typedly_def
-  proof
-    fix \<omega>
-    assume asm0: "\<omega> \<in> Set.filter (typed (make_context_semantic \<Delta> type_ctxt_front_end_syntactic)) (\<langle>\<Delta>, snd type_ctxt_front_end_syntactic\<rangle> \<Turnstile> \<langle>I\<rangle>) \<inter>
-             {\<omega> |\<omega>. bdenot b (get_store \<omega>)}"
-    moreover have "Some \<omega> = \<omega> \<oplus> |\<omega>|"
-      using core_is_smaller by auto
-    moreover have "TypedEqui.typed type_ctxt_front_end \<omega>"
-      by (metis IntD1 asm0 make_context_semantic_type_ctxt member_filter)
-    then have "|\<omega>| \<in> \<langle>\<Delta>, snd type_ctxt_front_end_syntactic\<rangle> \<Turnstile> \<langle>Atomic (Pure (translate_bexp b))\<rangle>"
-      using translation_correct_bexp[of _ _ b] asm0
-      unfolding sat_set.simps atomic_assert.simps red_pure_assert_def corely_def semantify_bexp_def make_semantic_bexp_def
-      by (metis (no_types, lifting) Int_iff TypedEqui.typed_core core_charact(1) core_in_emp_core mem_Collect_eq option.distinct(1) option.inject)
-    ultimately show "\<omega> \<in> Set.filter (typed (make_context_semantic \<Delta> type_ctxt_front_end_syntactic))
-               (\<langle>\<Delta>, snd type_ctxt_front_end_syntactic\<rangle> \<Turnstile> \<langle>I && Atomic (Pure (translate_bexp b))\<rangle>)"
-      using x_elem_set_product
-      by (smt (verit, ccfv_threshold) IntD1 member_filter sat_set.simps(4) snd_conv type_ctxt_front_end_syntactic_def)
-  qed
-qed
-*)
-(*
-lemma full_ownership_translation_sound:
-  "make_semantic_assertion \<Delta> type_ctxt_front_end_syntactic (Atomic (Acc (Var r) field_val (PureExp (ELit (LPerm 1)))))
-  = typed_stabilize (full_ownership r)"
-  unfolding make_semantic_assertion_def well_typedly_def full_ownership_def sat_set.simps atomic_assert.simps
-    TypedEqui.Stabilize_typed_def red_pure_assert_def corely_def emp_core_def
-  apply simp
-proof -
-  have "(\<Union>x xa xb.
-         \<Delta> \<turnstile> \<langle>Var r\<rangle> [\<Down>] Val (VRef x) \<otimes> \<llangle>snd type_ctxt_front_end_syntactic field_val = Some xb\<rrangle> \<otimes>
-         (\<Union>p'. \<Delta> \<turnstile> \<langle>ELit WritePerm\<rangle> [\<Down>] Val (VPerm p') \<otimes> \<llangle>xa = Some p'\<rrangle>) \<otimes>
-         acc \<Delta> xb x field_val xa) =
- (Stabilize {\<omega>. \<exists>l. get_store \<omega> r = Some (VRef (Address l)) \<and> get_m \<omega> (l, field_val) = 1})" (is "?A = ?B")
-  proof
-    show "?A \<subseteq> ?B"
-    proof
-      fix \<omega> assume asm0: "\<omega> \<in> ?A"
-      then obtain x xa xb where "\<omega> \<in> \<Delta> \<turnstile> \<langle>Var r\<rangle> [\<Down>] Val (VRef x) \<otimes> \<llangle>snd type_ctxt_front_end_syntactic field_val = Some xb\<rrangle> \<otimes>
-           (\<Union>p'. \<Delta> \<turnstile> \<langle>ELit WritePerm\<rangle> [\<Down>] Val (VPerm p') \<otimes> \<llangle>xa = Some p'\<rrangle>) \<otimes>
-           acc \<Delta> xb x field_val xa"
-        by (smt (z3) UN_iff snd_conv type_ctxt_front_end_syntactic_def)
-      then show "\<omega> \<in> ?B"
-        sorry
-    qed
-    show "?B \<subseteq> ?A"
-    proof
-      fix \<omega> assume asm0: "\<omega> \<in> ?B"
-      then obtain l where "get_store (stabilize \<omega>) r = Some (VRef (Address l))" "get_m (stabilize \<omega>) (l, field_val) = 1"
-        by auto
 
-      then show "\<omega> \<in> ?A" sorry
-    qed
-  qed
-  then show "Set.filter (typed tcfe)
-     (\<Union>x xa xb.
-         {\<omega>. \<Delta> \<turnstile> \<langle>Var r;\<omega>\<rangle> [\<Down>] Val (VRef x)} \<inter> Collect pure \<otimes> \<llangle>snd type_ctxt_front_end_syntactic field_val = Some xb\<rrangle> \<otimes>
-         (\<Union>p'. {\<omega>. \<Delta> \<turnstile> \<langle>ELit WritePerm;\<omega>\<rangle> [\<Down>] Val (VPerm p')} \<inter> Collect pure \<otimes> \<llangle>xa = Some p'\<rrangle>) \<otimes>
-         acc \<Delta> xb x field_val xa) =
-    Set.filter (typed tcfe) (Stabilize {\<omega>. \<exists>l. get_store \<omega> r = Some (VRef (Address l)) \<and> get_m \<omega> (l, field_val) = 1})"
-    unfolding red_pure_assert_def corely_def emp_core_def
-    by fastforce
-qed
-*)
 
-lemma full_ownership_with_val_sound:
-  "make_semantic_assertion \<Delta> F (Atomic (Acc (Var r) field_val (PureExp (ELit (LPerm 1)))) && Atomic (Pure (FieldAcc (Var r) field_val)))
-  = typed_stabilize (full_ownership_with_val r e)"
-  (* Does not hold if make_semantic_assertion does not use well_typedly*)
-  oops
+
+section \<open>The Translation\<close>
+
+
 
 
 fun translate_syn where
@@ -225,7 +426,7 @@ fun translate_syn where
 | "translate_syn \<Delta> F (Cassign x e) = (stmt.LocalAssign x (translate_exp e), {})"
 
 | "translate_syn \<Delta> F (Calloc r e) = ((stmt.Seq (stmt.Havoc r)
-  (stmt.Inhale (Atomic (Acc (Var r) field_val (PureExp (ELit (LPerm 1)))) && Atomic (Pure (FieldAcc (Var r) field_val))))), {})"
+  (stmt.Inhale (Atomic (Acc (Var r) field_val (PureExp (ELit (LPerm 1)))) && Atomic (Pure (Binop (FieldAcc (Var r) field_val) Eq (translate_exp e))))), {}))"
 
 | "translate_syn \<Delta> F (Cfree r) = (stmt.Exhale (Atomic (Acc (Var r) field_val (PureExp (ELit (LPerm 1))))), {})"
 
@@ -254,192 +455,675 @@ fun translate_syn where
   { stmt.Seq (stmt.Seq (stmt.Inhale (I && Atomic (Pure (translate_bexp b)))) (fst (translate_syn \<Delta> F C))) (stmt.Exhale I) }
   \<union> snd (translate_syn \<Delta> F C))"
 
-lemma havoc_list_n_havoc_same:
-  "compile \<Delta> F (n_havoc l) = ConcreteSemantics.havoc_list l"
-  by (induct l) simp_all
 
-thm ConcreteSemantics.verifies_set_def ConcreteSemantics.verifies_def
 
-inductive_simps ConcreteSemantics_red_stmt_simps :
-  "ConcreteSemantics.red_stmt \<Delta> (abs_stmt.LocalAssign x e) \<omega> S"
-  "ConcreteSemantics.red_stmt \<Delta> (abs_stmt.Exhale A) \<omega> S"
-  "ConcreteSemantics.red_stmt \<Delta> (abs_stmt.Inhale A) \<omega> S"
-  "ConcreteSemantics.red_stmt \<Delta> (C1;;C2) \<omega> S"
-  "ConcreteSemantics.red_stmt \<Delta> (Custom (custom.FieldAssign e1 f e2)) \<omega> S"
 
-lemma make_semantic_exp_implies_semantify_exp :
-  assumes "make_semantic_exp \<Delta> (translate_exp e) \<omega> = Some v"
-  assumes "typed tcfe \<omega>"
-  (* TODO: also needs to e has integer type *)
-  shows "semantify_exp e \<omega> = Some v"
-  using assms
-proof (induction e arbitrary:v)
-  case (Evar x)
-  then show ?case
-    apply (simp add:semantify_exp_def red_pure_simps)
-    sorry
-next
-  case (Elit x)
-  then show ?case by (simp add:semantify_exp_def red_pure_simps)
-next
-  case (Ebinop e1 op e2)
-  then show ?case
-    by (cases "op"; clarsimp simp add:semantify_exp_def red_pure_simps; fastforce)
+(* We want verification of the latter to imply verification of the former *)
+definition verifies_more_set:
+  "verifies_more_set \<Delta> S1 S2 \<longleftrightarrow> (\<forall>C1 \<in> S1. \<exists>C2 \<in> S2. verifies_more \<Delta> C1 C2)"
+
+lemma verifies_more_setI:
+  assumes "\<And>C1. C1 \<in> S1 \<Longrightarrow> (\<exists>C2 \<in> S2. verifies_more \<Delta> C1 C2)"
+  shows "verifies_more_set \<Delta> S1 S2"
+  by (simp add: assms verifies_more_set)
+
+lemma rel_stable_self_framing[simp]:
+  assumes "sep_algebra_class.stable \<omega>"
+      and "self_framing A"
+  shows "rel_stable_assertion \<omega> A"
+proof (rule rel_stable_assertionI)
+  fix \<omega>' a
+  assume asm0: "a \<in> A" "Some \<omega>' = \<omega> \<oplus> a"
+  then show "\<exists>a'\<in>A. Some (stabilize \<omega>') = \<omega> \<oplus> a'"
+    by (metis already_stable assms(1) assms(2) self_framingE stabilize_sum)
 qed
 
-lemma red_stmt_LocalAssign_mono :
-  assumes "ConcreteSemantics.red_stmt \<Gamma> (abs_stmt.LocalAssign x e1) \<omega> S"
-  assumes "\<And> v. e1 \<omega> = Some v \<Longrightarrow> e2 \<omega> = Some v"
-  shows "ConcreteSemantics.red_stmt \<Gamma> (abs_stmt.LocalAssign x e2) \<omega> S"
-  using assms by (clarsimp simp add:ConcreteSemantics_red_stmt_simps)
 
-lemma red_stmt_FieldAssign_mono :
-  assumes "ConcreteSemantics.red_stmt \<Gamma> (Custom (custom.FieldAssign e1 f e2)) \<omega> S"
-  assumes "\<And> v. e2 \<omega> = Some v \<Longrightarrow> e2' \<omega> = Some v"
-  shows "ConcreteSemantics.red_stmt \<Gamma> (Custom (custom.FieldAssign e1 f e2')) \<omega> S"
-  using assms by (clarsimp simp add:ConcreteSemantics_red_stmt_simps red_custom_stmt.simps)
 
-lemma red_stmt_Seq_mono :
-  assumes "ConcreteSemantics.red_stmt \<Gamma> (C1;;C2) \<omega> S"
-  assumes "\<And> S'. ConcreteSemantics.red_stmt \<Gamma> C1 \<omega> S' \<Longrightarrow> 
-       ConcreteSemantics.red_stmt \<Gamma> C1' \<omega> S' \<and> (\<forall> \<omega>' S''. \<omega>' \<in> S' \<longrightarrow>
-      ConcreteSemantics.red_stmt \<Gamma> C2 \<omega>' S'' \<longrightarrow> ConcreteSemantics.red_stmt \<Gamma> C2' \<omega>' S'')"
-  shows "ConcreteSemantics.red_stmt \<Gamma> (C1';;C2') \<omega> S"
-  using assms
-  apply (clarsimp simp add:ConcreteSemantics_red_stmt_simps ConcreteSemantics.sequential_composition.simps)
-  by blast
+lemma in_starE:
+  assumes "x \<in> A \<otimes> B"
+      and "\<And>a b. a \<in> A \<Longrightarrow> b \<in> B \<Longrightarrow> Some x = a \<oplus> b \<Longrightarrow> P"
+    shows "P"
+  by (meson assms(1) assms(2) x_elem_set_product)
 
-lemma red_stmt_Exhale_mono :
-  assumes "ConcreteSemantics.red_stmt \<Gamma> (abs_stmt.Exhale A1) \<omega> S"
-  assumes "\<And> \<omega>'. stable \<omega>' \<Longrightarrow> \<omega> \<in> {\<omega>'} \<otimes> A1 \<Longrightarrow> \<omega> \<in> {\<omega>'} \<otimes> A2"
-  shows "ConcreteSemantics.red_stmt \<Gamma> (abs_stmt.Exhale A2) \<omega> S"
-  using assms
-  apply (clarsimp simp add:ConcreteSemantics_red_stmt_simps add_set_def)
-  by blast
-
-lemma red_stmt_Inhale_mono :
-  assumes "ConcreteSemantics.red_stmt \<Gamma> (abs_stmt.Inhale A1) \<omega> S"
-  assumes "rel_stable_assertion \<omega> A1 \<Longrightarrow> rel_stable_assertion \<omega> A2"
-  assumes "Set.filter stable ({\<omega>} \<otimes> A1) = Set.filter stable ({\<omega>} \<otimes> A2)"
-  assumes "\<And> \<omega>'. stable \<omega>' \<Longrightarrow> \<omega> \<in> {\<omega>'} \<otimes> A1 \<Longrightarrow> \<omega> \<in> {\<omega>'} \<otimes> A2"
-  shows "ConcreteSemantics.red_stmt \<Gamma> (abs_stmt.Inhale A2) \<omega> S"
-  using assms
-  by (clarsimp simp add:ConcreteSemantics_red_stmt_simps)
-
-lemma translation_refines:
-  assumes "ConcreteSemantics.red_stmt tcfe (compile \<Delta> F (fst (translate_syn \<Delta> F C))) \<omega> S"
-      and "typed tcfe \<omega>"
-      and "stable \<omega>"
-(* need side condition on typing of program *)
-  shows "ConcreteSemantics.red_stmt tcfe (fst (translate \<Delta> C)) \<omega> S"
-  using assms
-proof (induct C arbitrary: \<omega> S)
-  case (Cassign x1 x2)
-  then show ?case
-    apply (simp)
-    apply (rule red_stmt_LocalAssign_mono) apply (assumption)
-    by (rule make_semantic_exp_implies_semantify_exp)
-next
-  case (Cwrite x1 x2)
-  then show ?case
-    apply (simp add:sound_translate_addr)
-    apply (rule red_stmt_FieldAssign_mono) apply (assumption)
-    by (rule make_semantic_exp_implies_semantify_exp)
-next
-  case (Calloc x1 x2)
-  then show ?case
-    apply (simp)
-    apply (rule red_stmt_Seq_mono) apply (assumption)
-    apply (rule) apply (assumption)
-    apply (rule; simp)
-    sorry
-next
-  case (Cfree x)
-  then show ?case
-    apply (simp)
-    apply (rule red_stmt_Exhale_mono) apply (assumption)
-    sorry
-next
-  case (Cseq C1 C2)
-  then show ?case
-    apply (simp add:)
-    sorry
-next
-  case (Cpar x1 C1 x3 x4 C2 x6a)
-  then show ?case sorry
-next
-  case (Cif x1 C1 C2)
-  then show ?case sorry
-next
-  case (Cwhile x1 x2 C)
-  then show ?case sorry
-qed (simp_all add: sound_translate_heap_loc)
 
 (*
-      and "ConcreteSemantics.verifies_set tcfe (atrue tcfe) (Inhale P;; fst (translate \<Gamma> C);; Exhale Q)"
-      and "\<And>Cv. Cv \<in> snd (translate \<Gamma> C) \<Longrightarrow> ConcreteSemantics.verifies_set tcfe (atrue tcfe) Cv"
+definition red_pure_assert ::  "('a, 'a virtual_state) interp \<Rightarrow> pure_exp \<Rightarrow> 'a extended_val \<Rightarrow> 'a equi_state set" ("_ \<turnstile> ((\<langle>_\<rangle>) [\<Down>] _)" [51,0,0] 81) where
+"red_pure_assert \<Delta> e r = corely {\<omega>. \<Delta> \<turnstile> \<langle>e; \<omega>\<rangle> [\<Down>] r}"
 *)
 
-(* main theorem *)
-(* does not hold since the sets are not actually equal *)
+lemma red_pure_varE:
+  assumes "\<Delta> \<turnstile> \<langle>Var r; \<omega>\<rangle> [\<Down>] Val v"
+      and "get_store \<omega> r = Some v \<Longrightarrow> P"
+    shows "P"
+  using RedVar2Val_case assms(1) assms(2) by blast
+
+
+lemma red_pure_litE:
+  assumes "\<Delta> \<turnstile> \<langle>ELit (LPerm p); \<omega>\<rangle> [\<Down>] Val (VPerm p')"
+      and "p = p' \<Longrightarrow> P"
+    shows "P"
+  using assms(1)
+  apply (rule red_pure_elim)
+  apply (simp add: assms(2))  
+  by simp
+
 (*
-lemma translation_same:
-  "compile \<Delta> F (fst (translate_syn \<Delta> F C)) = fst (translate \<Delta> C) \<and> compile \<Delta> F ` (snd (translate_syn \<Delta> F C)) = snd (translate \<Delta> C)"
+"emp = {a. \<exists> b. a = stabilize |b| }"
+*)
+lemma plus_emp_same:
+  assumes "Some \<omega> = stabilize |x| \<oplus> y"
+  shows "\<omega> = y"
+  by (simp add: assms commutative stabilize_core_emp)
+
+lemma in_emp_star_something:
+  assumes "x \<in> \<llangle>P\<rrangle> \<otimes> A"
+  shows "P \<and> x \<in> A"
+  by (metis add_set_commm add_set_empty_l assms bool_to_assertion_false bool_to_assertion_true emp_star_right_id emptyE)
+
+lemma in_something_star_emp:
+  assumes "x \<in> A \<otimes> \<llangle>P\<rrangle>"
+  shows "P \<and> x \<in> A"
+  by (metis add_set_commm add_set_empty_l assms bool_to_assertion_false bool_to_assertion_true emp_star_right_id emptyE)
+
+
+thm acc_heap_loc_starE
+
+lemma elim_in_acc_one:
+  assumes "b \<in> acc \<Delta> xb x field_val (Some 1)"
+  shows "get_m b (the_address x, field_val) = 1 \<and> (\<exists>v. x = Address v)"
+  using assms unfolding acc_def
+proof -
+  have "b \<in> (\<Union>pp. \<llangle>Some 1 = None \<or> pp = the (Some 1)\<rrangle> \<otimes> acc_heap_loc \<Delta> xb (the_address x, field_val) pp)"
+    by (smt (verit) Instantiation.acc_def Sup.SUP_cong assms bool_to_assertion_false empty_iff option.distinct(1) option.inject)
+  then obtain pp where "b \<in> \<llangle>pp = the (Some 1)\<rrangle> \<otimes> acc_heap_loc \<Delta> xb (the_address x, field_val) pp"
+    by force
+  then have "pp = 1 \<and> b \<in> acc_heap_loc \<Delta> xb (the_address x, field_val) pp"
+    using in_emp_star_something by auto
+  then have "get_m b (the_address x, field_val) = 1"
+    unfolding acc_heap_loc_def
+    apply simp
+    using one_preal.abs_eq by auto
+  moreover have "\<exists>v. x = Address v"
+    by (smt (verit, best) Instantiation.acc_def assms bool_to_assertion_false empty_iff option.sel ref.exhaust_sel)
+  ultimately show ?thesis by blast
+qed
+
+
+lemma sum_with_emp_simplifies:
+  assumes "b \<in> emp"
+      and "Some x = a \<oplus> b"
+    shows "x = a"
+  using assms(1) assms(2) is_in_set_sum by fastforce
+
+lemma verifies_more_free:
+  assumes "a \<in> make_semantic_assertion_untyped \<Delta> F (Atomic (Acc (Var r) field_val (PureExp (ELit WritePerm))))"
+    shows "a \<in> Stabilize (full_ownership r)"
+  apply (rule in_StabilizeI)
+  unfolding full_ownership_def
+  apply simp
+proof -
+  show "\<exists>l. get_store a r = Some (VRef (Address l)) \<and> get_m a (l, field_val) = 1"
+    using assms(1) unfolding make_semantic_assertion_gen_def
+    apply simp
+    apply (erule exE)+
+
+    apply (erule in_emp_star_something[elim_format] | erule in_something_star_emp[elim_format] | erule in_starE)+
+    apply simp
+    apply (erule exE)+
+    apply (erule in_emp_star_something[elim_format] | erule in_something_star_emp[elim_format] | erule in_starE)+
+
+    apply (simp add: red_pure_assert_def corely_def emp_core_def)
+    apply (erule conjE)+
+    apply (erule red_pure_varE)
+    apply (erule red_pure_litE)
+    apply simp
+    apply (erule elim_in_acc_one[elim_format])
+    by (metis (no_types, lifting) full_add_charact(1) greater_equiv larger_mask_full ref.sel)
+qed
+
+(* as long as no red_perm *)
+lemma red_pure_core_same:
+  assumes "\<Delta> \<turnstile> \<langle>e;\<omega>\<rangle> [\<Down>] r"
+  shows "\<Delta> \<turnstile> \<langle>e; |\<omega>| \<rangle> [\<Down>] r"
+  sorry
+
+
+lemma in_smth_star_red_pure_assertI:
+  assumes "\<Delta> \<turnstile> \<langle>e;\<omega>\<rangle> [\<Down>] r"
+      and "\<omega> \<in> A"
+    shows "\<omega> \<in> (\<Delta> \<turnstile> \<langle>e\<rangle> [\<Down>] r) \<otimes> A"
+proof -
+  have "|\<omega>| \<in> \<Delta> \<turnstile> \<langle>e\<rangle> [\<Down>] r"
+    unfolding red_pure_assert_def corely_def emp_core_def
+    apply simp
+    by (simp add: assms(1) core_is_pure pure_def red_pure_core_same)
+  then show ?thesis
+    using add_set_commm assms(2) core_is_smaller x_elem_set_product by blast
+qed
+
+lemma in_red_pure_assert_star_smthI:
+  assumes "\<Delta> \<turnstile> \<langle>e;\<omega>\<rangle> [\<Down>] r"
+      and "\<omega> \<in> A"
+    shows "\<omega> \<in> A \<otimes> (\<Delta> \<turnstile> \<langle>e\<rangle> [\<Down>] r)"
+  using add_set_commm assms(1) assms(2) in_smth_star_red_pure_assertI by blast
+
+
+lemma get_vh_stabilize_implies_normal:
+  assumes "get_vh (stabilize (get_state a)) hl = Some v"
+  shows "get_h a hl = Some v"
+  by (simp add: assms stabilize_value_persists)
+
+lemma typed_exp_then_value:
+  assumes "typed_exp e"
+      and "typed tcfe a"
+    shows "\<exists>v. \<Delta> \<turnstile> \<langle>translate_exp e;a\<rangle> [\<Down>] Val v"
+  sorry
+
+lemma verifies_more_alloc:
+  assumes "typed_exp e"
+      and "r \<in> dom (variables tcfe)"
+      and "TypedEqui.wf_assertion tcfe (Stabilize (full_ownership_with_val r e))"
+      and "typed tcfe a"
+      and "a \<in> Stabilize (full_ownership_with_val r e)"
+(* This translation is wrong... *)
+    shows "a \<in> make_semantic_assertion_untyped \<Delta> F (Atomic (Acc (Var r) field_val (PureExp (ELit WritePerm))) && Atomic (Pure (Binop (FieldAcc (Var r) field_val) Eq (translate_exp e))))"
+  using assms(5)
+  unfolding make_semantic_assertion_gen_def
+  apply simp unfolding full_ownership_with_val_def
+  apply simp
+  apply (erule exE)
+  apply (erule conjE)+
+  apply (rule in_red_pure_assert_star_smthI)
+  apply (rule RedBinop)
+  apply (rule RedField)
+      apply (rule RedVar)
+      apply simp_all
+     apply (erule get_vh_stabilize_implies_normal)
+    apply (rule exE[OF typed_exp_then_value[OF assms(1) assms(4), of \<Delta>]])
+  
+
+  apply (rule exI)
+
+  sorry
+
+
+(*
+  apply (rule in_StabilizeI)
+  unfolding full_ownership_def
+  apply simp
+proof -
+  show "\<exists>l. get_store a r = Some (VRef (Address l)) \<and> get_m a (l, field_val) = 1"
+    using assms(1) unfolding make_semantic_assertion_gen_def
+    apply simp
+    apply (erule exE)+
+
+    apply (erule in_emp_star_something[elim_format] | erule in_something_star_emp[elim_format] | erule in_starE)+
+    apply simp
+    apply (erule exE)+
+    apply (erule in_emp_star_something[elim_format] | erule in_something_star_emp[elim_format] | erule in_starE)+
+
+    apply (simp add: red_pure_assert_def corely_def emp_core_def)
+    apply (erule conjE)+
+    apply (erule red_pure_varE)
+    apply (erule red_pure_litE)
+    apply simp
+    apply (erule elim_in_acc_one[elim_format])
+    by (metis (no_types, lifting) full_add_charact(1) greater_equiv larger_mask_full ref.sel)
+qed
+
+*)
+
+
+
+
+
+
+(* TODO: Remove useless assumptions *)
+lemma verifies_more_translation_while_exhale:
+  assumes "(ConcreteSemantics.wf_abs_stmt tcfe (fst (translate \<Delta> C)) \<Longrightarrow>
+          verifies_more tcfe (fst (translate \<Delta> C)) (compile False \<Delta> F (fst (translate_syn \<Delta> F C))))"
+      and "typed_bexp b"
+      and "typed_stmt C"
+      and "TypedEqui.wf_assertion tcfe (inhalify (make_semantic_assertion_untyped \<Delta> type_ctxt_front_end_syntactic I))"
+      and "ConcreteSemantics.wf_abs_stmt tcfe (ConcreteSemantics.havoc_list (wrL C))"
+      and "TypedEqui.wf_assertion tcfe (make_semantic_assertion_untyped \<Delta> type_ctxt_front_end_syntactic I \<inter> assertify_bexp (Bnot b))"
+      and "typed tcfe a"
+      and "a \<in> make_semantic_assertion_untyped \<Delta> F I"
+    shows "a \<in> inhalify (make_semantic_assertion_untyped \<Delta> type_ctxt_front_end_syntactic I)"
+  sorry
+
+
+lemma verifies_more_translation_while_inhale:
+  assumes "(ConcreteSemantics.wf_abs_stmt tcfe (fst (translate \<Delta> C)) \<Longrightarrow>
+          verifies_more tcfe (fst (translate \<Delta> C)) (compile False \<Delta> F (fst (translate_syn \<Delta> F C))))"
+      and "typed_bexp b"
+      and "typed_stmt C"
+      and "TypedEqui.wf_assertion tcfe (inhalify (make_semantic_assertion_untyped \<Delta> type_ctxt_front_end_syntactic I))"
+      and "ConcreteSemantics.wf_abs_stmt tcfe (ConcreteSemantics.havoc_list (wrL C))"
+      and "TypedEqui.wf_assertion tcfe (make_semantic_assertion_untyped \<Delta> type_ctxt_front_end_syntactic I \<inter> assertify_bexp (Bnot b))"
+      and "typed tcfe a"
+      and "a \<in> make_semantic_assertion_untyped \<Delta> type_ctxt_front_end_syntactic I \<inter> assertify_bexp (Bnot b)"
+    shows "a \<in> make_semantic_assertion_untyped \<Delta> F (I && Atomic (Pure (Unop unop.Not (translate_bexp b))))"
+  sorry
+
+
+lemma verifies_more_translation_parallel_exhale:
+  assumes "(ConcreteSemantics.wf_abs_stmt tcfe (fst (translate \<Delta> C1)) \<Longrightarrow>
+          verifies_more tcfe (fst (translate \<Delta> C1)) (compile False \<Delta> F (fst (translate_syn \<Delta> F C1))))"
+      and "(ConcreteSemantics.wf_abs_stmt tcfe (fst (translate \<Delta> C2)) \<Longrightarrow>
+          verifies_more tcfe (fst (translate \<Delta> C2)) (compile False \<Delta> F (fst (translate_syn \<Delta> F C2))))"
+      and "typed_stmt C1"
+      and "typed_stmt C2"
+      and "TypedEqui.wf_assertion tcfe
+          (inhalify
+            (make_semantic_assertion_untyped \<Delta> type_ctxt_front_end_syntactic P1 \<otimes> make_semantic_assertion_untyped \<Delta> type_ctxt_front_end_syntactic P2))"
+      and "ConcreteSemantics.wf_abs_stmt tcfe (ConcreteSemantics.havoc_list (wrL C1 @ wrL C2))"
+      and "TypedEqui.wf_assertion tcfe
+          (make_semantic_assertion_untyped \<Delta> type_ctxt_front_end_syntactic Q1 \<otimes> make_semantic_assertion_untyped \<Delta> type_ctxt_front_end_syntactic Q2)"
+      and "typed tcfe a"
+      and "a \<in> make_semantic_assertion_untyped \<Delta> F (P1 && P2)"
+    shows "a \<in> inhalify
+               (make_semantic_assertion_untyped \<Delta> type_ctxt_front_end_syntactic P1 \<otimes> make_semantic_assertion_untyped \<Delta> type_ctxt_front_end_syntactic P2)"
+  sorry
+
+lemma verifies_more_translation_parallel_inhale:
+  assumes "(ConcreteSemantics.wf_abs_stmt tcfe (fst (translate \<Delta> C1)) \<Longrightarrow>
+          verifies_more tcfe (fst (translate \<Delta> C1)) (compile False \<Delta> F (fst (translate_syn \<Delta> F C1))))"
+      and "(ConcreteSemantics.wf_abs_stmt tcfe (fst (translate \<Delta> C2)) \<Longrightarrow>
+          verifies_more tcfe (fst (translate \<Delta> C2)) (compile False \<Delta> F (fst (translate_syn \<Delta> F C2))))"
+      and "typed_stmt C1"
+      and "typed_stmt C2"
+      and "TypedEqui.wf_assertion tcfe
+          (inhalify
+            (make_semantic_assertion_untyped \<Delta> type_ctxt_front_end_syntactic P1 \<otimes> make_semantic_assertion_untyped \<Delta> type_ctxt_front_end_syntactic P2))"
+      and "ConcreteSemantics.wf_abs_stmt tcfe (ConcreteSemantics.havoc_list (wrL C1 @ wrL C2))"
+      and "TypedEqui.wf_assertion tcfe
+          (make_semantic_assertion_untyped \<Delta> type_ctxt_front_end_syntactic Q1 \<otimes> make_semantic_assertion_untyped \<Delta> type_ctxt_front_end_syntactic Q2)"
+      and "typed tcfe a"
+      and "a \<in> make_semantic_assertion_untyped \<Delta> type_ctxt_front_end_syntactic Q1 \<otimes> make_semantic_assertion_untyped \<Delta> type_ctxt_front_end_syntactic Q2"
+    shows "a \<in> make_semantic_assertion_untyped \<Delta> F (Q1 && Q2)"
+  sorry
+
+lemma verifies_more_while_snd_exhale:
+  assumes "typed_stmt (Cwhile b I C)"
+      and "wf_stmt \<Delta> F (Cwhile b I C)"
+      and "TypedEqui.wf_assertion tcfe (make_semantic_assertion_untyped \<Delta> type_ctxt_front_end_syntactic I \<inter> assertify_bexp b)"
+      and "typed tcfe a"
+      and "a \<in> make_semantic_assertion_untyped \<Delta> type_ctxt_front_end_syntactic I \<inter> assertify_bexp b"
+    shows "a \<in> make_semantic_assertion_untyped \<Delta> F (I && Atomic (Pure (translate_bexp b)))"
+  sorry
+
+lemma verifies_more_while_snd_exhale_bis:
+  assumes "typed_stmt (Cwhile b I C)"
+      and "wf_stmt \<Delta> F (Cwhile b I C)"
+      and "TypedEqui.wf_assertion tcfe (make_semantic_assertion_untyped \<Delta> type_ctxt_front_end_syntactic I \<inter> assertify_bexp b)"
+      and "typed tcfe a"
+      and "a \<in> make_semantic_assertion_untyped \<Delta> F I"
+    shows "a \<in> inhalify (make_semantic_assertion_untyped \<Delta> type_ctxt_front_end_syntactic I)"
+  sorry
+
+
+
+lemma n_havoc_same:
+  "ConcreteSemantics.havoc_list l = compile False \<Delta> F (n_havoc l)"
+  by (induct l) simp_all
+
+lemma self_framing_inter[simp]:
+  assumes "self_framing A"
+  shows "self_framing (A \<inter> assertify_bexp b)"
+proof (rule self_framingI)
+  fix \<omega>   
+  show "(\<omega> \<in> A \<inter> assertify_bexp b) = (stabilize \<omega> \<in> A \<inter> assertify_bexp b)"
+  proof -
+    have "\<omega> \<in> assertify_bexp b \<longleftrightarrow> stabilize \<omega> \<in> assertify_bexp b"
+      by (simp add: assertify_bexp_def)
+    then show ?thesis
+      using assms self_framing_def by auto
+  qed
+qed
+
+
+
+
+
+lemma translation_refinement_main:
+  assumes "typed_stmt C"
+      and "ConcreteSemantics.wf_abs_stmt tcfe (fst (translate \<Delta> C))"
+      and "wf_stmt \<Delta> F C"
+(* TODO: Understand the type contexts of verifies_more, translate, compile, translate_syn *)
+  shows "verifies_more tcfe (fst (translate \<Delta> C)) (compile False \<Delta> F (fst (translate_syn \<Delta> F C)))"
+  using assms
 proof (induct C)
-  case (Cassign x1 x2)
-  then show ?case using translation_correct_exp compile.simps(5) translate.simps(2) translate_syn.simps(2)
+  case Cskip
+  then show ?case by simp
+next
+  case (Cassign x e)
+  then show ?case
+    apply simp
+    apply (rule verifies_more_local_assign[of tcfe "semantify_exp e" "make_semantic_exp \<Delta> (translate_exp e)" x])
+    apply (rule exp_refined_by_int[of e \<Delta>])
     by simp
 next
   case (Cread x1 x2)
-  then show ?case unfolding translate.simps translate_syn.simps
-    using sound_translate_heap_loc by force
+  then show ?case
+    by (simp add: sound_translate_heap_loc)
 next
-  case (Cwrite x1 x2)
-  then show ?case unfolding translate.simps translate_syn.simps
-    using sound_translate_addr translation_correct_exp by auto
+  case (Cwrite r e)
+  then show ?case
+    apply simp
+    apply (rule verifies_more_field_assign)
+    apply (simp add: sound_translate_addr)
+    using exp_refined_by_int by blast
 next
-  case (Calloc x1 x2)
-  then show ?case unfolding translate.simps translate_syn.simps
-    by (simp add: full_ownership_with_val_sound)
+  case (Calloc r e)
+  then show ?case
+    apply simp
+    apply (rule verifies_more_seq)
+    apply simp_all
+    apply (rule verifies_more_inhale)
+     apply simp
+    using verifies_more_alloc by blast
 next
-  case (Cfree x)
-  then show ?case unfolding translate.simps translate_syn.simps
-    using full_ownership_translation_sound by force
+  case (Cfree r)
+  then show ?case
+    apply simp
+    apply (rule verifies_more_exhale)
+    using verifies_more_free by blast
 next
   case (Cseq C1 C2)
   then show ?case
-    by (metis compile.simps(3) fst_eqD image_Un snd_eqD translate.simps(7) translate_syn.simps(7))
-next
-  case (Cpar x1 C1 x3 x4 C2 x6a)
-  show ?case
-  proof
-    show "compile \<Delta> F (fst (translate_syn \<Delta> F {x1} C1 {x3} || {x4} C2 {x6a})) = fst (translate \<Delta> F {x1} C1 {x3} || {x4} C2 {x6a})"
-      unfolding translate.simps translate_syn.simps
-      by (simp add: havoc_list_n_havoc_same make_semantic_star)
-    show "compile \<Delta> F ` snd (translate_syn \<Delta> F {x1} C1 {x3} || {x4} C2 {x6a}) = snd (translate \<Delta> F {x1} C1 {x3} || {x4} C2 {x6a})"
-      unfolding translate.simps translate_syn.simps 
-      apply (simp add: make_semantic_star)
-      by (metis Cpar.hyps(1) Cpar.hyps(2) compile.simps(3) compile.simps(6) compile.simps(7) image_Un image_insert)
+    apply simp
+  proof -
+    assume asm0: "ConcreteSemantics.wf_abs_stmt tcfe (fst (translate \<Delta> C1)) \<Longrightarrow> verifies_more tcfe (fst (translate \<Delta> C1)) (compile False \<Delta> F (fst (translate_syn \<Delta> F C1)))"
+      "ConcreteSemantics.wf_abs_stmt tcfe (fst (translate \<Delta> C2)) \<Longrightarrow> verifies_more tcfe (fst (translate \<Delta> C2)) (compile False \<Delta> F (fst (translate_syn \<Delta> F C2)))"
+      "typed_stmt C1 \<and> typed_stmt C2"
+    have "verifies_more tcfe (fst (translate \<Delta> C1) ;; fst (translate \<Delta> C2))
+     (Seq (compile False \<Delta> F (fst (translate_syn \<Delta> F C1))) (compile False \<Delta> F (fst (translate_syn \<Delta> F C2))))"
+      apply (rule verifies_more_seq)
+      using asm0
+      apply (metis ConcreteSemantics.wf_abs_stmt.simps(7) Cseq.prems(2) fst_eqD translate.simps(7))
+       apply (metis ConcreteSemantics.wf_abs_stmt.simps(7) Cseq.prems(2) asm0(2) fst_eqD translate.simps(7))
+      by (metis ConcreteSemantics.wf_abs_stmt.simps(7) Cseq.prems(2) fst_eqD translate.simps(7))
+    then show "verifies_more tcfe (fst (let r1 = translate \<Delta> C1; r2 = translate \<Delta> C2 in (fst r1 ;; fst r2, snd r1 \<union> snd r2)))
+     (compile False \<Delta> F (fst (let r1 = translate_syn \<Delta> F C1; r2 = translate_syn \<Delta> F C2 in (stmt.Seq (fst r1) (fst r2), snd r1 \<union> snd r2))))"
+      by (metis compile.simps(3) fst_eqD)
   qed
 next
-  case (Cif x1 C1 C2)
-  then show ?case unfolding translate.simps translate_syn.simps
-    by (simp add: image_Un translation_correct_bexp)
+  case (Cpar P1 C1 Q1 P2 C2 Q2)
+  then show ?case
+    apply simp
+    apply (rule verifies_more_seq)
+    apply (rule verifies_more_seq)
+    apply (rule verifies_more_exhale)
+    using verifies_more_translation_parallel_exhale apply blast
+    apply (metis n_havoc_same verifies_more_refl)
+    apply auto[1]
+     apply (rule verifies_more_inhale)
+      apply (rule rel_stable_self_framing)
+    apply simp
+      apply (rule typed_self_framing_star)
+       apply simp_all
+    using verifies_more_translation_parallel_inhale by blast
 next
-  case (Cwhile x1 x2 C)
+  case (Cif b C1 C2)
+  then show ?case
+    apply simp
+    apply (rule verifies_more_if)
+    apply blast
+    apply meson
+    using bexp_refined_by by blast
+next
+  case (Cwhile b I C)
+  then show ?case
+    apply simp
+    apply (rule verifies_more_seq)
+      apply (rule verifies_more_seq)
+    apply (rule verifies_more_exhale)    
+    using verifies_more_translation_while_exhale apply blast
+       apply (metis n_havoc_same verifies_more_refl)
+    using ConcreteSemantics.wf_abs_stmt.simps(3) apply blast
+     apply (rule verifies_more_inhale)
+      apply (rule rel_stable_self_framing)
+       apply simp_all
+    by (meson IntI verifies_more_translation_while_inhale)
+qed
+
+
+lemma simplified_snd_if[simp]:
+  "snd (translate \<Delta> (Cif b C1 C2)) = snd (translate \<Delta> C1) \<union> snd (translate \<Delta> C2)"
+  by simp
+
+
+abbreviation tcfes where
+  "tcfes \<equiv> type_ctxt_front_end_syntactic"
+
+
+
+
+lemma translation_refinement_snd:
+  assumes "typed_stmt C"
+      and "wf_stmt \<Delta> tcfes C"
+      and "\<And>Cv. Cv \<in> snd (translate \<Delta> C) \<Longrightarrow> ConcreteSemantics.wf_abs_stmt tcfe Cv"
+      and "ConcreteSemantics.wf_abs_stmt tcfe (fst (translate \<Delta> C))"
+      and "Csem \<in> snd (translate \<Delta> C)"
+    shows "\<exists>Csyn \<in> snd (translate_syn \<Delta> tcfes C). verifies_more tcfe Csem (compile False \<Delta> tcfes Csyn)"
+  using assms
+proof (induct C arbitrary: )
+  case (Cseq C1 C2)
   show ?case
-  proof
-    show "compile \<Delta> F (fst (translate_syn \<Delta> F (Cwhile x1 x2 C))) = fst (translate \<Delta> F (Cwhile x1 x2 C))"
-      unfolding translate.simps translate_syn.simps
-      by (simp add: havoc_list_n_havoc_same make_semantic_inter_1)
-    show "compile \<Delta> F ` snd (translate_syn \<Delta> F (Cwhile x1 x2 C)) = snd (translate \<Delta> F (Cwhile x1 x2 C))"
-      unfolding translate.simps translate_syn.simps
-      apply (simp add: havoc_list_n_havoc_same make_semantic_inter_2)
-      using Cwhile by presburger
+  proof (cases "Csem \<in> snd (translate \<Delta> C1)")
+    case True
+    have "\<exists>Csyn\<in>snd (translate_syn \<Delta> tcfes C1). verifies_more tcfe Csem (compile False \<Delta> tcfes Csyn)"
+      apply (rule Cseq(1))
+      using Cseq.prems(1) apply fastforce
+      using Cseq.prems(2) apply force
+         apply (metis Cseq.prems(3) Un_iff snd_conv translate.simps(7))
+        apply (metis ConcreteSemantics.wf_abs_stmt.simps(7) Cseq.prems(4) fst_eqD translate.simps(7))
+      by (auto simp add: True Cseq)
+    then show ?thesis
+      by (metis Un_iff snd_conv translate_syn.simps(7))
+  next
+    case False
+    have "\<exists>Csyn\<in>snd (translate_syn \<Delta> tcfes C2). verifies_more tcfe Csem (compile False \<Delta> tcfes Csyn)"
+      apply (rule Cseq(2))
+      using Cseq.prems(1) apply fastforce
+      using Cseq.prems(2) apply force
+         apply (metis Cseq.prems(3) Un_iff snd_conv translate.simps(7))
+      apply (metis ConcreteSemantics.wf_abs_stmt.simps(7) Cseq.prems(4) fst_eqD translate.simps(7))
+      by (metis Cseq.prems(5) False Un_iff snd_conv translate.simps(7))
+    then show ?thesis
+      by (metis Un_iff snd_conv translate_syn.simps(7))
+  qed
+next
+  case (Cpar P1 C1 Q1 P2 C2 Q2)
+  then show ?case
+    apply (cases "Csem \<in> snd (translate \<Delta> C1)")
+     apply simp
+     apply (metis (no_types, lifting) ConcreteSemantics.wf_abs_stmt.simps(7) Un_iff insertCI)
+    apply (cases "Csem \<in> snd (translate \<Delta> C2)")
+     apply simp
+     apply (metis (no_types, lifting) ConcreteSemantics.wf_abs_stmt.simps(7) Un_iff insertCI)
+
+  proof -
+
+    let ?P1 = "make_semantic_assertion_untyped \<Delta> type_ctxt_front_end_syntactic P1"
+    let ?Q1 = "make_semantic_assertion_untyped \<Delta> type_ctxt_front_end_syntactic Q1"
+    let ?P2 = "make_semantic_assertion_untyped \<Delta> type_ctxt_front_end_syntactic P2"
+    let ?Q2 = "make_semantic_assertion_untyped \<Delta> type_ctxt_front_end_syntactic Q2"
+
+    assume asm0: "typed_stmt ({P1} C1 {Q1} || {P2} C2 {Q2})" "wf_stmt \<Delta> tcfes ({P1} C1 {Q1} || {P2} C2 {Q2})"
+      "\<And>Cv. Cv \<in> snd (translate \<Delta> {P1} C1 {Q1} || {P2} C2 {Q2}) \<Longrightarrow> ConcreteSemantics.wf_abs_stmt tcfe Cv"
+      "Csem \<in> snd (translate \<Delta> {P1} C1 {Q1} || {P2} C2 {Q2})" "Csem \<notin> snd (translate \<Delta> C1)"
+    "Csem \<notin> snd (translate \<Delta> C2)" "ConcreteSemantics.wf_abs_stmt tcfe (fst (translate \<Delta> {P1} C1 {Q1} || {P2} C2 {Q2}))"
+
+
+    then have "Csem = (Inhale ?P1;; fst (translate \<Delta> C1);; Exhale (inhalify ?Q1)) \<or> Csem = (Inhale ?P2;; fst (translate \<Delta> C2);; Exhale (inhalify ?Q2))"
+      using asm0 translate.simps(9)[of \<Delta> P1 C1 Q1 P2 C2 Q2]
+      by (simp add: Let_def)
+
+
+    moreover have "verifies_more tcfe (Inhale ?P1;; fst (translate \<Delta> C1);; Exhale (inhalify ?Q1)) (compile False \<Delta> tcfes (stmt.Seq (stmt.Seq (stmt.Inhale P1) (fst (translate_syn \<Delta> tcfes C1))) (stmt.Exhale Q1)))"
+      apply simp
+      apply (rule verifies_more_seq)
+      apply (rule verifies_more_seq)
+          apply (rule verifies_more_inhale)
+      using asm0(2) apply fastforce
+      using assms(5) apply blast
+         apply (rule translation_refinement_main)
+      using asm0 apply simp_all
+         apply (simp add: Let_def)
+      using asm0(7)
+      apply (metis ConcreteSemantics.wf_abs_stmt.simps(7))
+      using asm0
+      apply (meson ConcreteSemantics.wf_abs_stmt.simps(2) ConcreteSemantics.wf_abs_stmt.simps(7) insertCI)
+       apply (simp add: Let_def)
+       apply (rule verifies_more_exhale)
+       apply (simp add: TypedEqui.typed_state_then_stabilize_typed)
+      by (meson ConcreteSemantics.wf_abs_stmt.simps(2) ConcreteSemantics.wf_abs_stmt.simps(7) insertI1)
+
+    moreover have "verifies_more tcfe (Inhale ?P2;; fst (translate \<Delta> C2);; Exhale (inhalify ?Q2))
+    (compile False \<Delta> tcfes (stmt.Seq (stmt.Seq (stmt.Inhale P2) (fst (translate_syn \<Delta> tcfes C2))) (stmt.Exhale Q2)))"
+      apply simp
+      apply (rule verifies_more_seq)
+      apply (rule verifies_more_seq)
+          apply (rule verifies_more_inhale)
+      using asm0(2) apply fastforce
+      using assms(5) apply blast
+         apply (rule translation_refinement_main)
+      using asm0 apply simp_all
+         apply (simp add: Let_def)
+      using asm0(7)
+      apply (metis ConcreteSemantics.wf_abs_stmt.simps(7))
+      using asm0
+      apply (meson ConcreteSemantics.wf_abs_stmt.simps(2) ConcreteSemantics.wf_abs_stmt.simps(7) insertCI)
+       apply (simp add: Let_def)
+       apply (rule verifies_more_exhale)
+       apply (simp add: TypedEqui.typed_state_then_stabilize_typed)
+      by (meson ConcreteSemantics.wf_abs_stmt.simps(2) ConcreteSemantics.wf_abs_stmt.simps(7) insertCI)
+    ultimately show "\<exists>Csyn\<in>snd (translate_syn \<Delta> tcfes {P1} C1 {Q1} || {P2} C2 {Q2}). verifies_more tcfe Csem (compile False \<Delta> tcfes Csyn)"
+      unfolding translate_syn.simps Let_def
+      by force
+  qed
+next
+  case (Cif b C1 C2)
+  then show ?case
+    apply (cases "Csem \<in> snd (translate \<Delta> C1)")
+    apply simp
+    using Cif(1) Cif.prems translate_syn.simps(8)[of \<Delta> tcfes b C1 C2]
+     apply blast
+    apply simp
+    using Cif(2) Cif.prems translate_syn.simps(8)[of \<Delta> tcfes b C1 C2]
+    by blast
+next
+  case (Cwhile b I C)
+  then show ?case
+    apply (cases "Csem \<in> snd (translate \<Delta> C)")
+     apply simp
+     apply fastforce
+  proof -
+    assume asm0: "typed_stmt (Cwhile b I C)" "wf_stmt \<Delta> tcfes (Cwhile b I C)"
+    "\<And>Cv. Cv \<in> snd (translate \<Delta> (Cwhile b I C)) \<Longrightarrow> ConcreteSemantics.wf_abs_stmt tcfe Cv"
+    "Csem \<in> snd (translate \<Delta> (Cwhile b I C))" "Csem \<notin> snd (translate \<Delta> C)"
+
+    let ?I = "make_semantic_assertion_untyped \<Delta> type_ctxt_front_end_syntactic I"
+
+    have r: "Csem = Inhale (?I \<inter> assertify_bexp b);; fst (translate \<Delta> C);; Exhale (inhalify ?I)"
+      using asm0 by simp
+
+    have "verifies_more tcfe (Inhale (?I \<inter> assertify_bexp b);; fst (translate \<Delta> C);; Exhale (inhalify ?I))
+  (compile False \<Delta> tcfes (stmt.Seq (stmt.Seq (stmt.Inhale (I && Atomic (Pure (translate_bexp b)))) (fst (translate_syn \<Delta> tcfes C))) (stmt.Exhale I)))"
+      apply simp
+      apply (rule verifies_more_seq)
+      apply (rule verifies_more_seq)
+          apply (rule verifies_more_inhale)
+      using asm0(2) apply auto[1]
+      using verifies_more_while_snd_exhale[of b I C \<Delta> tcfes]
+      apply (metis ConcreteSemantics.wf_abs_stmt.simps(2) ConcreteSemantics.wf_abs_stmt.simps(7) asm0(1) asm0(2) asm0(3) asm0(4) r)
+         apply (rule translation_refinement_main)      
+      using asm0(1) apply auto[1]
+      using ConcreteSemantics.wf_abs_stmt.simps(7) assms(3) assms(5) r apply blast
+      using asm0(2) apply force
+      using ConcreteSemantics.wf_abs_stmt.simps(7) asm0(3) asm0(4) r apply blast
+       apply (rule verifies_more_exhale)
+      apply (metis ConcreteSemantics.wf_abs_stmt.simps(7) asm0(1) asm0(2) asm0(3) asm0(4) r ConcreteSemantics.wf_abs_stmt.simps(2) verifies_more_while_snd_exhale_bis)
+      using ConcreteSemantics.wf_abs_stmt.simps(7) asm0(3) asm0(4) r
+      by blast
+    then show "\<exists>Csyn\<in>snd (translate_syn \<Delta> tcfes (Cwhile b I C)). verifies_more tcfe Csem (compile False \<Delta> tcfes Csyn)"
+      using asm0 by simp
   qed
 qed (simp_all)
-*)
 
+
+theorem translation_refinement_syntactic_semantic:
+  assumes "typed_stmt C"
+      and "wf_stmt \<Delta> tcfes C"
+      and "ConcreteSemantics.wf_abs_stmt tcfe (fst (translate \<Delta> C))"
+      and "\<And>Cv. Cv \<in> snd (translate \<Delta> C) \<Longrightarrow> ConcreteSemantics.wf_abs_stmt tcfe Cv"
+    shows "verifies_more tcfe (fst (translate \<Delta> C)) (compile False \<Delta> tcfes (fst (translate_syn \<Delta> tcfes C)))"
+      and "verifies_more_set tcfe (snd (translate \<Delta> C)) (compile False \<Delta> tcfes ` (snd (translate_syn \<Delta> tcfes C)))"
+  using assms(1) assms(2) assms(3) translation_refinement_main apply blast
+  apply (rule verifies_more_setI)
+  using translation_refinement_snd[OF assms(1) assms(2) assms(4) assms(3)]
+  by (metis image_eqI)
+
+
+lemma verifies_more_verifies:
+  assumes "verifies_more \<Delta> C C'"
+      and "ConcreteSemantics.verifies \<Delta> C' \<omega>"
+      and "typed \<Delta> \<omega>"
+      and "stable \<omega>"
+    shows "ConcreteSemantics.verifies \<Delta> C \<omega>"
+  by (meson ConcreteSemantics.verifies_def assms(1) assms(2) assms(3) assms(4) verifies_moreE)
+
+
+theorem sound_syntactic_translation:
+
+(* Well formedness *)
+
+  assumes "wf_stmt \<Delta> tcfes C"
+      and "well_typed_cmd tcfe C"
+      and "ConcreteSemantics.wf_abs_stmt tcfe (fst (translate \<Delta> C))"
+      and "\<And>Cv. Cv \<in> snd (translate \<Delta> C) \<Longrightarrow> ConcreteSemantics.wf_abs_stmt tcfe Cv"
+      and "TypedEqui.wf_assertion tcfe P \<and> TypedEqui.wf_assertion tcfe Q"
+      and "typed_stmt C" (* TODO: Unify the two notions of typing *)
+
+(* Verification *)
+      and "ConcreteSemantics.verifies_set tcfe atrue (abs_stmt.Inhale P ;; compile False \<Delta> tcfes (fst (translate_syn \<Delta> tcfes C)) ;; abs_stmt.Exhale Q)"
+      and "\<And>Cv. Cv \<in> compile False \<Delta> tcfes ` (snd (translate_syn \<Delta> tcfes C)) \<Longrightarrow> ConcreteSemantics.verifies_set tcfe atrue Cv"
+
+shows "tcfe \<turnstile>CSL [P \<otimes> UNIV] C [Q \<otimes> UNIV]"
+  using assms(1) assms(2) assms(3) assms(4) assms(5)
+proof (rule sound_translation)
+  show "ConcreteSemantics.verifies_set tcfe atrue (abs_stmt.Inhale P ;; fst (translate \<Delta> C) ;; abs_stmt.Exhale Q)"
+  proof (rule ConcreteSemantics.verifies_setI)
+    fix \<omega> assume asm0: "\<omega> \<in> atrue" "sep_algebra_class.stable \<omega>" "typed tcfe \<omega>"
+    show "ConcreteSemantics.verifies tcfe (abs_stmt.Inhale P ;; fst (translate \<Delta> C) ;; abs_stmt.Exhale Q) \<omega>"
+    proof (rule verifies_more_verifies)
+      show "verifies_more tcfe (abs_stmt.Inhale P ;; fst (translate \<Delta> C) ;; abs_stmt.Exhale Q)
+      (abs_stmt.Inhale P ;; compile False \<Delta> tcfes (fst (translate_syn \<Delta> tcfes C)) ;; abs_stmt.Exhale Q)"
+        apply (rule verifies_more_seq)
+        apply (rule verifies_more_seq)
+            apply simp_all
+        using translation_refinement_main
+        using assms(1) assms(3) assms(6) apply blast
+        apply (simp add: assms(5))
+        using assms(3) assms(5) by blast
+
+      show "ConcreteSemantics.verifies tcfe (abs_stmt.Inhale P ;; compile False \<Delta> tcfes (fst (translate_syn \<Delta> tcfes C)) ;; abs_stmt.Exhale Q) \<omega>"
+        using ConcreteSemantics.verifies_set_def asm0(1) asm0(2) asm0(3) assms(7) by blast
+    qed (simp_all add: asm0)
+  qed
+  fix Cv
+  assume asm0: "Cv \<in> snd (translate \<Delta> C)"
+  moreover have "verifies_more_set tcfe (snd (translate \<Delta> C)) (compile False \<Delta> tcfes ` (snd (translate_syn \<Delta> tcfes C)))"
+    using assms(1) assms(3) assms(4) assms(6) translation_refinement_syntactic_semantic(2) by blast
+  ultimately obtain Cv' where "Cv' \<in> compile False \<Delta> tcfes ` (snd (translate_syn \<Delta> tcfes C))"
+    "verifies_more tcfe Cv Cv'"
+    by (meson verifies_more_set)
+  then show "ConcreteSemantics.verifies_set tcfe atrue Cv"
+    by (meson ConcreteSemantics.verifies_set_def assms(8) verifies_more_verifies)
+qed (simp_all)
 
 
 end
